examples/ring/CellIAproof.v
@@ -32,8 +32,8 @@ Section SIMMODSEM.
 
   Variable idx: nat.
   
-  Variable StbA: Sk.t -> gname -> option fspec.
-  Hypothesis CellInStb: forall sk, stb_incl (to_stb (CellAS.Stb idx)) (StbA sk).
+  Variable StbG: Sk.t -> gname -> option fspec.
+  Hypothesis CellInStb: forall sk, stb_incl (CellAS.Stb idx) (StbG sk).
 
   Import CellAS.
 
@@ -62,97 +62,83 @@ Section SIMMODSEM.
   Proof.
   Admitted.
 
-  Definition Ist: Any.t -> Any.t -> iProp :=
-    (fun st_src st_tgt =>
-       ∃ v,
-       (cell idx v ∗ auth idx v)
-       ∨ 
-       (pending idx ∗ auth idx v ∗ ⌜st_tgt = v↑⌝))%I.
-  
-  Local Notation CellAMod := (CellA.t idx StbA).
+  Definition Ist: Sk.t -> alist key Any.t -> alist key Any.t -> iProp :=
+    (fun _ st_src st_tgt =>
+       ∃vany v, ⌜st_tgt = [(CellI.v_cv idx, vany)]⌝ ∗
+       ((cell idx v ∗ auth idx v)
+        ∨
+        (⌜vany = v↑⌝ ∗ pending idx ∗ auth idx v)))%I.
+
   Local Notation CellIMod := (CellI.t idx).
-
-  (* Lemma simF_init: *)
-  (*   HModR.sim_fun CellAMod CellIMod Ist (CellName.init idx). *)
-  (* Proof. *)
-  (*   init_simF. *)
-
-  (*   st_l. iDestruct "ASM" as "((% & P) & %)". *)
-  (*   subst. hss. unfold Ist. *)
-  (*   iDestruct "IST" as "[(C & A) | (P' & _)]"; des; subst; cycle 1. *)
-  (*   { iExFalso. iApply (pending_unique with "P' P"). } *)
-
-  (*   st_r. force_l. st_l. force_l. force_l. *)
-  (*   iSplitL "C". *)
-  (*   { eauto. } *)
-
-  (*   st. *)
-  (*   iSplitL; eauto. *)
-  (*   iRight. iFrame. eauto. *)
-  (* Qed. *)
+  Local Notation CellAMod := (CellA.t idx StbG (const emp%I)).
 
   Lemma simF_get:
     HModR.sim_fun CellAMod CellIMod Ist (CellName.get idx).
   Proof.
     init_simF.
 
-    st_l. iDestruct "ASM" as "((% & C) & %)".
-    subst. hss. rename y0 into v. unfold Ist.
-    iDestruct "IST" as (v')"[(C0 & _)|(P & A & %)]".
-    { iExFalso. iApply (cell_unique with "C0 C"). }
+    steps_l. iDestruct "ASM" as "((% & C) & %)".
+    subst. hss. rename q into v. unfold Ist.
+    iDestruct "IST" as (vany v0) "(% & [(C' & A)|(% & P & A)])".
+    { iExFalso. iApply (cell_unique with "C' C"). }
     subst. hss.
 
     iPoseProof (cell_auth_get with "C A") as "%". subst.
 
-    st_r. force_l. st_l. force_l. force_l.
+    steps_r. hss. steps_r.    
+    apc_l. steps_l.
+    force_l. steps_l. force_l. force_l.
     iSplitL "C". { eauto. }
 
-    st. iSplitL; [|eauto].
-    iExists _. iRight. iFrame. eauto.
+    step. iSplitL; [|eauto].
+    iExists _, _. iSplitL ""; eauto. iRight. iFrame; eauto.
   Qed.
   
   Lemma simF_set:
     HModR.sim_fun CellAMod CellIMod Ist (CellName.set idx).
   Proof.
     init_simF.
-    
-    st_l. hss. iDestruct "ASM" as "((% & [P|C]) & %)"; subst; hss.
-    { iDestruct "IST" as (v')"[(C & A)|(P' & A & %)]"; des; subst; cycle 1.
-      { iExFalso. iApply (pending_unique with "P' P"). }
 
-      iPoseProof (cell_auth_get with "C A") as "%". subst.
+    steps_l. iDestruct "ASM" as "((% & [P|C]) & %)";
+      subst; hss; rename q0 into v, q1 into v'; unfold Ist.
+    { iDestruct "IST" as (vany v0) "(% & [(C & A)|(% & P' & A)])"; cycle 1.
+      { iExFalso. iApply (pending_unique with "P' P"). }
+      des; subst. hss.
+      
       iMod (cell_auth_set with "C A") as "(C & A)".
 
-      st_r. force_l. st_l. force_l. force_l.
+      steps_r. hss.
+      apc_l. steps_l. force_l. steps_l. force_l. force_l.
       iSplitL "C". { eauto. }
 
-      st.
+      step.
       iSplitL; eauto.
-      iExists _. iRight. iFrame. eauto.
+      iExists _, _. iSplitL ""; eauto. iRight. iFrame; eauto.
     }
-      
-    iDestruct "IST" as (v')"[(C' & A)|(P & A & %)]".
+
+    iDestruct "IST" as (vany v0) "(% & [(C' & A)|(% & P & A)])".
     { iExFalso. iApply (cell_unique with "C' C"). }
     subst. hss.
 
     iPoseProof (cell_auth_get with "C A") as "%". subst.
     iMod (cell_auth_set with "C A") as "(C & A)".
-    
-    st_r. force_l. st_l. force_l. force_l.
+
+    steps_r. hss.
+    apc_l. steps_l. force_l. steps_l. force_l. force_l.
     iSplitL "C". { eauto. }
 
-    st. iSplitL; [|eauto].
-    iExists _. iRight. iFrame. eauto.
+    step.
+    iSplitL; [|eauto].
+    iExists _, _. iSplitL ""; eauto. iRight. iFrame; eauto.
   Qed.
 
   Theorem sim: HModR.sim CellAMod CellIMod Ist.
   Proof.
     init_sim.
-    - iIntros "X". iDestruct "X" as (v) "(C & A)".
-      iSplitL ""; eauto.
-      unfold Ist. iExists _. iLeft. iFrame.
-    - use_simF simF_get.
-    - use_simF simF_set.
+    - iIntros "H". iDestruct "H" as (v) "(C & A & E)". iFrame.
+      repeat iExists _. iSplitL ""; eauto. iLeft. iFrame.
+    - apply simF_get.
+    - apply simF_set.
   Qed.
 
 End SIMMODSEM.
