simulations/isim/ISimCore.v
@@ -16,6 +16,7 @@ Require Import Red IRed.
 Require Import HPSim.
 Require Import World sWorld.
 Require Import Red IRed.
+Require Import SubPerm.
 
 From stdpp Require Import coPset gmap.
 (* Require Import FancyUpdate. *)
@@ -783,105 +784,6 @@ End SIM.
 
 Global Opaque isim.
 
-Definition sub_perm {A} (l1 l2: list A) : Prop :=
-  exists l0, (l0 ++ l1) ≡ₚ l2.
-
-Lemma sub_perm_incl {A} (l1 l2: list A)
-  (SP: sub_perm l1 l2)
-  :
-  incl l1 l2.
-Proof.
-  r in SP. des.
-  ii. eapply Permutation_in; eauto.
-  apply in_or_app. eauto.
-Qed.
-
-Lemma sub_perm_nodup {A} (l1 l2: list A)
-  (SP: sub_perm l1 l2)
-  (ND: List.NoDup l2)
-  :
-  List.NoDup l1.
-Proof.
-  r in SP. des.
-  eapply Permutation_NoDup in ND; cycle 1.
-  - symmetry. eauto.
-  - eapply nodup_app_r. eauto.
-Qed.
-
-Lemma sub_perm_cancel {A} (l0 l1 l1' l2 l2': list A)
-  (SP: sub_perm (l1 ++ l2) (l1' ++ l2'))
-  :
-  sub_perm (l1 ++ l0 ++ l2) (l1' ++ l0 ++ l2').
-Proof.
-  r in SP. des. exists l3.
-  do 2 rewrite Permutation_app_rot.
-  rewrite <-!app_assoc. symmetry.
-  rewrite Permutation_app_rot.
-  apply Permutation_app_head.
-  rewrite Permutation_app_comm. symmetry.
-  rewrite Permutation_app_rot. eauto.
-Qed.
-
-Lemma sub_perm_cancel_head {A} (l0 l l': list A)
-  (SP: sub_perm l l')
-  :
-  sub_perm (l0 ++ l) (l0 ++ l').
-Proof.
-  apply (sub_perm_cancel l0 [] []). eauto.
-Qed.
-
-Lemma sub_perm_cancel_tail {A} (l0 l l': list A)
-  (SP: sub_perm l l')
-  :
-  sub_perm (l ++ l0) (l' ++ l0).
-Proof.
-  assert (X:=sub_perm_cancel l0 l l' [] []).
-  rewrite !app_nil_r in *. eauto.
-Qed.
-
-Lemma sub_perm_remove {A} (l0 l1 l2: list A):
-  sub_perm (l1 ++ l2) (l1 ++ l0 ++ l2).
-Proof.
-  exists l0.
-  rewrite/__ !List.app_assoc [l0 ++ _]Permutation_app_comm.
-  eauto.
-Qed.
-
-Lemma sub_perm_remove_head {A} (l0 l: list A):
-  sub_perm l (l0 ++ l).
-Proof.
-  apply (sub_perm_remove l0 []).
-Qed.
-
-Lemma sub_perm_remove_tail {A} (l0 l: list A):
-  sub_perm l (l ++ l0).
-Proof.
-  assert (X := sub_perm_remove l0 l []).
-  rewrite !app_nil_r in *. eauto.
-Qed.
-
-Lemma sub_perm_refl {A} (l: list A):
-  sub_perm l l.
-Proof.
-  apply (sub_perm_remove_head []).
-Qed.
-
-Lemma sub_perm_trans {A} (l1 l2 l3: list A):
-  sub_perm l1 l2 -> sub_perm l2 l3 -> sub_perm l1 l3.
-Proof.
-  unfold sub_perm. i; des.
-  eexists. rewrite/__ -H0 -H.
-  rewrite app_assoc. eauto.
-Qed.
-
-Lemma sub_perm_nil {A} (l: list A):
-  sub_perm [] l.
-Proof.
-  apply (sub_perm_remove_tail l []).
-Qed.
-
-
-
 Module HModSemR.
   Section SIM.
     Import HModSem.
@@ -895,8 +797,8 @@ Module HModSemR.
     Let fnsems_tgt := ms_tgt.(fnsems).
     Let init_src := ms_src.(initial_st).
     Let init_tgt := ms_tgt.(initial_st).
-    Let cond_src := HModSem.to_iprop (ms_src.(initial_cond)).
-    Let cond_tgt := HModSem.to_iprop (ms_tgt.(initial_cond)).
+    Let cond_src := ms_src.(initial_cond).
+    Let cond_tgt := ms_tgt.(initial_cond).
 
     Definition sim_fun fn : Prop :=
       forall
@@ -912,15 +814,18 @@ Module HModSemR.
 
     Inductive sim: Prop :=
       mk {
-          sim_initial: cond_src ⊢ cond_tgt ∗ (Ist init_src init_tgt);
-          sim_scopes: sub_perm scopes_tgt scopes_src; 
-          (* sim_scopes: incl scopes_tgt scopes_src; *)
-          (* sim_nodup: List.NoDup scopes_src -> List.NoDup scopes_tgt; *)
-          sim_length: List.length fnsems_src = List.length fnsems_tgt;
-          sim_miss: 
-            forall fn (MISS: alist_find fn fnsems_src = None),
-              alist_find fn fnsems_tgt = None;
-          sim_fnsems: forall fn, sim_fun fn;
+          sim_initial:
+            cond_src ⊢ cond_tgt ∗ (Ist init_src init_tgt);
+          sim_scopes:
+            sub_perm scopes_tgt scopes_src; 
+          sim_length:
+            List.length fnsems_src = List.length fnsems_tgt;
+          sim_match:
+            forall fn (IN: In fn (List.map fst fnsems_tgt)),
+              In fn (List.map fst fnsems_src);
+          sim_fnsems:
+            forall fn (IN: In fn (List.map fst fnsems_src)),
+              sim_fun fn;
         }.
 
   End SIM.
